WIP -- faced problem with permission

demo/owned_heap/BoxSource.v
@@ -13,8 +13,8 @@ Set Implicit Arguments.
 
 Local Obligation Tactic := ii; ss; des; inv_all_once; repeat des_u; ss; clarify.
 
-Definition update V (map: block -> option V) (k0: block) (v: V): block -> option V :=
-  fun k1 => if eq_block k0 k1 then Some v else map k1.
+Definition update V (map: block -> option V) (k0: block) (v: option V): block -> option V :=
+  fun k1 => if eq_block k0 k1 then v else map k1.
 
 Definition lo:Z := -8.
 Definition hi:Z := 4.
@@ -40,6 +40,9 @@ Section MODSEM.
       (k: block)
       (v: int)
       (oh: owned_heap) (m: mem)
+  | CallstateDelete
+      (k: block)
+      (oh: owned_heap) (m: mem)
   | ReturnstateNew
       (k: block)
       (oh: owned_heap) (m: mem)
@@ -47,6 +50,8 @@ Section MODSEM.
       (v: int)
       (oh: owned_heap) (m: mem)
   | ReturnstateSet
+      (oh: owned_heap) (m: mem)
+  | ReturnstateDelete
       (oh: owned_heap) (m: mem)
   .
 
@@ -81,6 +86,15 @@ Section MODSEM.
       (M: (Args.m args) = m)
     :
       initial_frame oh args (CallstateSet key val oh m)
+  | initial_frame_delete
+      (WF: oh_wf oh)
+      m blk key
+      (SYMB: Genv.find_symbol skenv _delete = Some blk)
+      (FPTR: (Args.fptr args) = Vptr blk Ptrofs.zero)
+      (VS: (Args.vs args) = [Vptr key Ptrofs.zero])
+      (M: (Args.m args) = m)
+    :
+      initial_frame oh args (CallstateDelete key oh m)
   .
 
   Inductive step (se: Senv.t) (ge: SkEnv.t): state -> trace -> state -> Prop :=
@@ -88,7 +102,7 @@ Section MODSEM.
       oh0 m0 oh1 m1 m2 key val
       (ALLOC: Mem.alloc m0 lo hi = (m1, key))
       (FREE: Mem.free m1 key lo hi = Some m2)
-      (OH: update oh0 key val = oh1)
+      (OH: update oh0 key (Some val) = oh1)
     :
       step se ge (CallstateNew val oh0 m0) E0 (ReturnstateNew key oh1 m2)
   | step_get
@@ -99,9 +113,15 @@ Section MODSEM.
   | step_set
       oh0 m key val oh1
       (SOME: oh0 key <> None)
-      (SET: update oh0 key val = oh1)
+      (SET: update oh0 key (Some val) = oh1)
     :
       step se ge (CallstateSet key val oh0 m) E0 (ReturnstateSet oh1 m)
+  | step_delete
+      oh0 m key oh1
+      (SOME: oh0 key <> None)
+      (SET: update oh0 key None = oh1)
+    :
+      step se ge (CallstateDelete key oh0 m) E0 (ReturnstateDelete oh1 m)
   .
 
   Inductive final_frame: state -> owned_heap -> Retv.t -> Prop :=
@@ -117,6 +137,10 @@ Section MODSEM.
       oh m
     :
       final_frame (ReturnstateSet oh m) oh (Retv.mk Vundef m)
+  | final_delete
+      oh m
+    :
+      final_frame (ReturnstateDelete oh m) oh (Retv.mk Vundef m)
   .
 
   Program Definition modsem: ModSem.t :=
