demo/owned_heap/MemoryC2.v
@@ -1,0 +1,536 @@
+Require Import Zwf.
+Require Import Axioms.
+Require Import CoqlibC.
+Require Intv.
+Require Import MapsC.
+Require Archi.
+Require Import ASTC.
+Require Import IntegersC.
+Require Import Floats.
+Require Import ValuesC.
+Require Export Memdata MemdataC.
+Require Export Memtype.
+Require Import sflib.
+Require Import Lia.
+Require Import Events.
+Require Import Classical_Pred_Type.
+Require Import Coq.Logic.FunctionalExtensionality.
+
+Local Notation "a # b" := (PMap.get b a) (at level 1).
+
+
+Require Export Memory.
+
+Module Mem.
+  Include Memory.Mem.
+  Local Transparent load.
+  Local Transparent loadbytes.
+
+  Definition perm_kind_dec (k0 k1: perm_kind): {k0 = k1} + {k0 <> k1}.
+    decide equality.
+  Defined.
+
+  Section FREEWEAK.
+    Program Definition unchecked_free_weak (m: mem) (b: block) (lo hi: Z): mem :=
+      Mem.mkmem m.(Mem.mem_contents)
+                    (PMap.set b
+                              (fun ofs k => if zle lo ofs && zlt ofs hi && perm_kind_dec k Cur
+                                            then None
+                                            else m.(Mem.mem_access)#b ofs k)
+                              m.(Mem.mem_access))
+                    m.(Mem.nextblock) _ _ _.
+    Next Obligation.
+      repeat rewrite PMap.gsspec. destruct (peq b0 b).
+      - r. des_ifs; bsimpl; des; des_sumbool; ss.
+        + exploit Mem.access_max; eauto. rewrite Heq. rewrite Heq0. ii; ss.
+        + exploit Mem.access_max; eauto. rewrite Heq. rewrite Heq0. ii; ss.
+        + exploit Mem.access_max; eauto. rewrite Heq. rewrite Heq0. ii; ss.
+        + exploit Mem.access_max; eauto. rewrite Heq. rewrite Heq0. ii; ss.
+      - apply Mem.access_max.
+    Qed.
+    Next Obligation.
+      repeat rewrite PMap.gsspec. destruct (peq b0 b).
+      - subst.
+        des_ifs; auto. apply Mem.nextblock_noaccess; auto.
+      - apply Mem.nextblock_noaccess; auto.
+    Qed.
+    Next Obligation.
+      apply Mem.contents_default.
+    Qed.
+    Definition free_weak (m: mem) (b: block) (lo hi: Z): option mem :=
+      if Mem.range_perm_dec m b lo hi Cur Freeable
+      then Some(unchecked_free_weak m b lo hi)
+      else None.
+  End FREEWEAK.
+
+  Theorem range_perm_free_weak:
+    forall m1 b lo hi,
+      range_perm m1 b lo hi Cur Freeable ->
+      { m2: mem | free_weak m1 b lo hi = Some m2 }.
+  Proof.
+    intros; unfold free_weak. rewrite pred_dec_true; auto. econstructor; eauto.
+  Defined.
+
+  Section FREE_WEAK.
+
+    Variable m1: mem.
+    Variable bf: block.
+    Variables lo hi: Z.
+    Variable m2: mem.
+    Hypothesis FREE_WEAK: free_weak m1 bf lo hi = Some m2.
+
+    Theorem free_weak_range_perm:
+      range_perm m1 bf lo hi Cur Freeable.
+    Proof.
+      unfold free_weak in FREE_WEAK. destruct (range_perm_dec m1 bf lo hi Cur Freeable); auto.
+      congruence.
+    Qed.
+
+    Lemma free_weak_result:
+      m2 = unchecked_free_weak m1 bf lo hi.
+    Proof.
+      unfold free_weak in FREE_WEAK. destruct (range_perm_dec m1 bf lo hi Cur Freeable).
+      congruence. congruence.
+    Qed.
+
+    Theorem nextblock_free_weak:
+      nextblock m2 = nextblock m1.
+    Proof.
+      rewrite free_weak_result; reflexivity.
+    Qed.
+
+    Theorem valid_block_free_weak_1:
+      forall b, valid_block m1 b -> valid_block m2 b.
+    Proof.
+      intros. rewrite free_weak_result. assumption.
+    Qed.
+
+    Theorem valid_block_free_weak_2:
+      forall b, valid_block m2 b -> valid_block m1 b.
+    Proof.
+      intros. rewrite free_weak_result in H. assumption.
+    Qed.
+
+    Local Hint Resolve valid_block_free_weak_1 valid_block_free_weak_2: mem.
+
+    Theorem perm_free_weak_1:
+      forall b ofs k p,
+        b <> bf \/ ofs < lo \/ hi <= ofs ->
+        perm m1 b ofs k p ->
+        perm m2 b ofs k p.
+    Proof.
+      intros. rewrite free_weak_result. unfold perm, unchecked_free_weak; simpl.
+      rewrite PMap.gsspec. destruct (peq b bf). subst b.
+      destruct (zle lo ofs); simpl.
+      destruct (zlt ofs hi); simpl.
+      elimtype False; intuition.
+      auto. auto.
+      auto.
+    Qed.
+
+    Theorem perm_free_weak_2:
+      forall ofs p, lo <= ofs < hi -> ~ perm m2 bf ofs Cur p.
+    Proof.
+      intros. rewrite free_weak_result. unfold perm, unchecked_free_weak; simpl.
+      rewrite PMap.gss. unfold proj_sumbool. rewrite zle_true. rewrite zlt_true.
+      simpl. tauto. omega. omega.
+    Qed.
+
+    Theorem perm_free_weak_3:
+      forall b ofs k p,
+        perm m2 b ofs k p -> perm m1 b ofs k p.
+    Proof.
+      intros until p. rewrite free_weak_result. unfold perm, unchecked_free_weak; simpl.
+      rewrite PMap.gsspec. destruct (peq b bf). subst b.
+      destruct (zle lo ofs); simpl.
+      destruct (zlt ofs hi); simpl. des_ifs.
+      auto. auto. auto.
+    Qed.
+
+    Theorem perm_free_weak_inv:
+      forall b ofs k p,
+        perm m1 b ofs k p ->
+        (b = bf /\ lo <= ofs < hi) \/ perm m2 b ofs k p.
+    Proof.
+      intros. rewrite free_weak_result. unfold perm, unchecked_free_weak; simpl.
+      rewrite PMap.gsspec. destruct (peq b bf); auto. subst b.
+      destruct (zle lo ofs); simpl; auto.
+      destruct (zlt ofs hi); simpl; auto.
+    Qed.
+
+    Theorem valid_access_free_weak_1:
+      forall chunk b ofs p,
+        valid_access m1 chunk b ofs p ->
+        b <> bf \/ lo >= hi \/ ofs + size_chunk chunk <= lo \/ hi <= ofs ->
+        valid_access m2 chunk b ofs p.
+    Proof.
+      intros. inv H. constructor; auto with mem.
+      red; intros. eapply perm_free_weak_1; eauto.
+      destruct (zlt lo hi). intuition. right. omega.
+    Qed.
+
+    Theorem valid_access_free_weak_2:
+      forall chunk ofs p,
+        lo < hi -> ofs + size_chunk chunk > lo -> ofs < hi ->
+        ~(valid_access m2 chunk bf ofs p).
+    Proof.
+      intros; red; intros. inv H2.
+      generalize (size_chunk_pos chunk); intros.
+      destruct (zlt ofs lo).
+      elim (perm_free_weak_2 lo p).
+      omega. apply H3. omega.
+      elim (perm_free_weak_2 ofs p).
+      omega. apply H3. omega.
+    Qed.
+
+    Theorem valid_access_free_weak_inv_1:
+      forall chunk b ofs p,
+        valid_access m2 chunk b ofs p ->
+        valid_access m1 chunk b ofs p.
+    Proof.
+      intros. destruct H. split; auto.
+      red; intros. generalize (H ofs0 H1).
+      rewrite free_weak_result. unfold perm, unchecked_free_weak; simpl.
+      rewrite PMap.gsspec. destruct (peq b bf). subst b.
+      destruct (zle lo ofs0); simpl.
+      destruct (zlt ofs0 hi); simpl.
+      tauto. auto. auto. auto.
+    Qed.
+
+    Theorem valid_access_free_weak_inv_2:
+      forall chunk ofs p,
+        valid_access m2 chunk bf ofs p ->
+        lo >= hi \/ ofs + size_chunk chunk <= lo \/ hi <= ofs.
+    Proof.
+      intros.
+      destruct (zlt lo hi); auto.
+      destruct (zle (ofs + size_chunk chunk) lo); auto.
+      destruct (zle hi ofs); auto.
+      elim (valid_access_free_weak_2 chunk ofs p); auto. omega.
+    Qed.
+
+    Theorem load_free_weak:
+      forall chunk b ofs,
+        b <> bf \/ lo >= hi \/ ofs + size_chunk chunk <= lo \/ hi <= ofs ->
+        load chunk m2 b ofs = load chunk m1 b ofs.
+    Proof.
+      intros. unfold load.
+      destruct (valid_access_dec m2 chunk b ofs Readable).
+      rewrite pred_dec_true.
+      rewrite free_weak_result; auto.
+      eapply valid_access_free_weak_inv_1; eauto.
+      rewrite pred_dec_false; auto.
+      red; intro; elim n. eapply valid_access_free_weak_1; eauto.
+    Qed.
+
+    Theorem load_free_weak_2:
+      forall chunk b ofs v,
+        load chunk m2 b ofs = Some v -> load chunk m1 b ofs = Some v.
+    Proof.
+      intros. unfold load. rewrite pred_dec_true.
+      rewrite (load_result _ _ _ _ _ H). rewrite free_weak_result; auto.
+      apply valid_access_free_weak_inv_1. eauto with mem.
+    Qed.
+
+    Theorem loadbytes_free_weak:
+      forall b ofs n,
+        b <> bf \/ lo >= hi \/ ofs + n <= lo \/ hi <= ofs ->
+        loadbytes m2 b ofs n = loadbytes m1 b ofs n.
+    Proof.
+      intros. unfold loadbytes.
+      destruct (range_perm_dec m2 b ofs (ofs + n) Cur Readable).
+      rewrite pred_dec_true.
+      rewrite free_weak_result; auto.
+      red; intros. eapply perm_free_weak_3; eauto.
+      rewrite pred_dec_false; auto.
+      red; intros. elim n0; red; intros.
+      eapply perm_free_weak_1; eauto. destruct H; auto. right; omega.
+    Qed.
+
+    Theorem loadbytes_free_weak_2:
+      forall b ofs n bytes,
+        loadbytes m2 b ofs n = Some bytes -> loadbytes m1 b ofs n = Some bytes.
+    Proof.
+      intros. unfold loadbytes in *.
+      destruct (range_perm_dec m2 b ofs (ofs + n) Cur Readable); inv H.
+      rewrite pred_dec_true. rewrite free_weak_result; auto.
+      red; intros. apply perm_free_weak_3; auto.
+    Qed.
+
+  End FREE_WEAK.
+
+  Local Hint Resolve valid_block_free_weak_1 valid_block_free_weak_2
+        perm_free_weak_1 perm_free_weak_2 perm_free_weak_3
+        valid_access_free_weak_1 valid_access_free_weak_inv_1: mem.
+
+  Lemma free_weak_left_inj:
+    forall f m1 m2 b lo hi m1',
+      mem_inj f m1 m2 ->
+      free_weak m1 b lo hi = Some m1' ->
+      mem_inj f m1' m2.
+  Proof.
+    intros. exploit free_weak_result; eauto. intro FREE_WEAK. inversion H. constructor.
+    (* perm *)
+    intros. eauto with mem.
+    (* align *)
+    intros. eapply mi_align0 with (ofs := ofs) (p := p); eauto.
+    red; intros; eapply perm_free_weak_3; eauto.
+    (* mem_contents *)
+    intros. rewrite FREE_WEAK; simpl. eauto with mem.
+  Qed.
+
+  Lemma free_weak_right_inj:
+    forall f m1 m2 b lo hi m2',
+      mem_inj f m1 m2 ->
+      free_weak m2 b lo hi = Some m2' ->
+      (forall b' delta ofs k p,
+          f b' = Some(b, delta) ->
+          perm m1 b' ofs k p -> lo <= ofs + delta < hi -> False) ->
+      mem_inj f m1 m2'.
+  Proof.
+    intros. exploit free_weak_result; eauto. intro FREE_WEAK. inversion H.
+    assert (PERM:
+              forall b1 b2 delta ofs k p,
+                f b1 = Some (b2, delta) ->
+                perm m1 b1 ofs k p -> perm m2' b2 (ofs + delta) k p).
+    intros.
+    intros. eapply perm_free_weak_1; eauto.
+    destruct (eq_block b2 b); auto. subst b. right.
+    assert (~ (lo <= ofs + delta < hi)). red; intros; eapply H1; eauto.
+    omega.
+    constructor.
+    (* perm *)
+    auto.
+    (* align *)
+    eapply mi_align0; eauto.
+    (* mem_contents *)
+    intros. rewrite FREE_WEAK; simpl. eauto.
+  Qed.
+
+  (* Theorem free_weak_left_extends: *)
+  (*   forall m1 m2 b lo hi m1', *)
+  (*     extends m1 m2 -> *)
+  (*     free_weak m1 b lo hi = Some m1' -> *)
+  (*     extends m1' m2. *)
+  (* Proof. *)
+  (*   intros. inv H. constructor. *)
+  (*   rewrite (nextblock_free_weak _ _ _ _ _ H0). auto. *)
+  (*   eapply free_weak_left_inj; eauto. *)
+  (*   intros. exploit mext_perm_inv0; eauto. intros [A|A]. *)
+  (*   eapply perm_free_weak_inv in A; eauto. destruct A as [[A B]|A]; auto. *)
+  (*   subst b0. right; eapply perm_free_weak_2; eauto. *)
+  (*   intuition eauto using perm_free_weak_3. *)
+  (* Qed. *)
+
+  Theorem free_weak_right_extends:
+    forall m1 m2 b lo hi m2',
+      extends m1 m2 ->
+      free_weak m2 b lo hi = Some m2' ->
+      (forall ofs k p, perm m1 b ofs k p -> lo <= ofs < hi -> False) ->
+      extends m1 m2'.
+  Proof.
+    intros. inv H. constructor.
+    rewrite (nextblock_free_weak _ _ _ _ _ H0). auto.
+    eapply free_weak_right_inj; eauto.
+    unfold inject_id; intros. inv H. eapply H1; eauto. omega.
+    intros. eauto using perm_free_weak_3.
+  Qed.
+
+  Theorem free_weak_parallel_extends:
+    forall m1 m2 b lo hi m1',
+      extends m1 m2 ->
+      free_weak m1 b lo hi = Some m1' ->
+      exists m2',
+        free_weak m2 b lo hi = Some m2'
+        /\ extends m1' m2'.
+  Proof.
+    intros. inversion H.
+    assert ({ m2': mem | free_weak m2 b lo hi = Some m2' }).
+    apply range_perm_free_weak. red; intros.
+    replace ofs with (ofs + 0) by omega.
+    eapply perm_inj with (b1 := b); eauto.
+    eapply free_weak_range_perm; eauto.
+    destruct X as [m2' FREE_WEAK]. exists m2'; split; auto.
+    constructor.
+    rewrite (nextblock_free_weak _ _ _ _ _ H0).
+    rewrite (nextblock_free_weak _ _ _ _ _ FREE_WEAK). auto.
+    eapply free_weak_right_inj with (m1 := m1'); eauto.
+    eapply free_weak_left_inj; eauto.
+    unfold inject_id; intros. inv H1.
+    eapply perm_free_weak_2. eexact H0. instantiate (1 := ofs); omega. eauto.
+    intros. exploit mext_perm_inv0; eauto using perm_free_weak_3. intros [A|A].
+    eapply perm_free_weak_inv in A; eauto. destruct A as [[A B]|A]; auto.
+    subst b0. right; eapply perm_free_weak_2; eauto.
+    right; intuition eauto using perm_free_weak_3.
+  Qed.
+
+  Lemma free_weak_left_inject:
+    forall f m1 m2 b lo hi m1',
+      inject f m1 m2 ->
+      free_weak m1 b lo hi = Some m1' ->
+      inject f m1' m2.
+  Proof.
+    intros. inversion H. constructor.
+    (* inj *)
+    eapply free_weak_left_inj; eauto.
+    (* free_weakblocks *)
+    eauto with mem.
+    (* mappedblocks *)
+    auto.
+    (* no overlap *)
+    red; intros. eauto with mem.
+    (* representable *)
+    intros. eapply mi_representable0; try eassumption.
+    destruct H2; eauto with mem.
+    (* perm inv *)
+    intros. exploit mi_perm_inv0; eauto. intuition eauto using perm_free_weak_3.
+    eapply perm_free_weak_inv in H4; eauto. destruct H4 as [[A B] | A]; auto.
+    subst b1. right; eapply perm_free_weak_2; eauto.
+  Qed.
+
+  Lemma free_weak_right_inject:
+    forall f m1 m2 b lo hi m2',
+      inject f m1 m2 ->
+      free_weak m2 b lo hi = Some m2' ->
+      (forall b1 delta ofs k p,
+          f b1 = Some(b, delta) -> perm m1 b1 ofs k p ->
+          lo <= ofs + delta < hi -> False) ->
+      inject f m1 m2'.
+  Proof.
+    intros. inversion H. constructor.
+    (* inj *)
+    eapply free_weak_right_inj; eauto.
+    (* free_weakblocks *)
+    auto.
+    (* mappedblocks *)
+    eauto with mem.
+    (* no overlap *)
+    auto.
+    (* representable *)
+    auto.
+    (* perm inv *)
+    intros. eauto using perm_free_weak_3.
+  Qed.
+
+  Theorem free_weak_inject:
+    forall f m1 l m1' m2 b lo hi m2',
+      inject f m1 m2 ->
+      free_weak_list m1 l = Some m1' ->
+      free_weak m2 b lo hi = Some m2' ->
+      (forall b1 delta ofs k p,
+          f b1 = Some(b, delta) ->
+          perm m1 b1 ofs k p -> lo <= ofs + delta < hi ->
+          exists lo1, exists hi1, In (b1, lo1, hi1) l /\ lo1 <= ofs < hi1) ->
+      inject f m1' m2'.
+  Proof.
+    intros.
+    eapply free_weak_right_inject; eauto.
+    eapply free_weak_list_left_inject; eauto.
+    intros. exploit perm_free_weak_list; eauto. intros [A B].
+    exploit H2; eauto. intros [lo1 [hi1 [C D]]]. eauto.
+  Qed.
+
+  Theorem free_weak_parallel_inject:
+    forall f m1 m2 b lo hi m1' b' delta,
+      inject f m1 m2 ->
+      free_weak m1 b lo hi = Some m1' ->
+      f b = Some(b', delta) ->
+      exists m2',
+        free_weak m2 b' (lo + delta) (hi + delta) = Some m2'
+        /\ inject f m1' m2'.
+  Proof.
+    intros.
+    destruct (range_perm_free_weak m2 b' (lo + delta) (hi + delta)) as [m2' FREE_WEAK].
+    eapply range_perm_inject; eauto. eapply free_weak_range_perm; eauto.
+    exists m2'; split; auto.
+    eapply free_weak_inject with (m1 := m1) (l := (b,lo,hi)::nil); eauto.
+    simpl; rewrite H0; auto.
+    intros. destruct (eq_block b1 b).
+    subst b1. rewrite H1 in H2; inv H2.
+    exists lo, hi; split; auto with coqlib. omega.
+    exploit mi_no_overlap. eexact H. eexact n. eauto. eauto.
+    eapply perm_max. eapply perm_implies. eauto. auto with mem.
+    instantiate (1 := ofs + delta0 - delta).
+    apply perm_cur_max. apply perm_implies with Free_Weakable; auto with mem.
+    eapply free_weak_range_perm; eauto. omega.
+    intros [A|A]. congruence. omega.
+  Qed.
+
+  Lemma free_weak_unchanged_on:
+    forall m b lo hi m',
+      free_weak m b lo hi = Some m' ->
+      (forall i, lo <= i < hi -> ~ P b i) ->
+      unchanged_on m m'.
+  Proof.
+    intros; constructor; intros.
+    - rewrite (nextblock_free_weak _ _ _ _ _ H). apply Ple_refl.
+    - split; intros.
+      eapply perm_free_weak_1; eauto.
+      destruct (eq_block b0 b); auto. destruct (zlt ofs lo); auto. destruct (zle hi ofs); auto.
+      subst b0. elim (H0 ofs). omega. auto.
+      eapply perm_free_weak_3; eauto.
+    - unfold free_weak in H. destruct (range_perm_dec m b lo hi Cur Free_Weakable); inv H.
+      simpl. auto.
+  Qed.
+
+Global Opaque Mem.alloc Mem.free_weak Mem.store Mem.load Mem.storebytes Mem.loadbytes.
+
+Hint Resolve
+  Mem.valid_not_valid_diff
+  Mem.perm_implies
+  Mem.perm_cur
+  Mem.perm_max
+  Mem.perm_valid_block
+  Mem.range_perm_implies
+  Mem.range_perm_cur
+  Mem.range_perm_max
+  Mem.valid_access_implies
+  Mem.valid_access_valid_block
+  Mem.valid_access_perm
+  Mem.valid_access_load
+  Mem.load_valid_access
+  Mem.loadbytes_range_perm
+  Mem.valid_access_store
+  Mem.perm_store_1
+  Mem.perm_store_2
+  Mem.nextblock_store
+  Mem.store_valid_block_1
+  Mem.store_valid_block_2
+  Mem.store_valid_access_1
+  Mem.store_valid_access_2
+  Mem.store_valid_access_3
+  Mem.storebytes_range_perm
+  Mem.perm_storebytes_1
+  Mem.perm_storebytes_2
+  Mem.storebytes_valid_access_1
+  Mem.storebytes_valid_access_2
+  Mem.nextblock_storebytes
+  Mem.storebytes_valid_block_1
+  Mem.storebytes_valid_block_2
+  Mem.nextblock_alloc
+  Mem.alloc_result
+  Mem.valid_block_alloc
+  Mem.fresh_block_alloc
+  Mem.valid_new_block
+  Mem.perm_alloc_1
+  Mem.perm_alloc_2
+  Mem.perm_alloc_3
+  Mem.perm_alloc_4
+  Mem.perm_alloc_inv
+  Mem.valid_access_alloc_other
+  Mem.valid_access_alloc_same
+  Mem.valid_access_alloc_inv
+  Mem.range_perm_free_weak
+  Mem.free_weak_range_perm
+  Mem.nextblock_free_weak
+  Mem.valid_block_free_weak_1
+  Mem.valid_block_free_weak_2
+  Mem.perm_free_weak_1
+  Mem.perm_free_weak_2
+  Mem.perm_free_weak_3
+  Mem.valid_access_free_weak_1
+  Mem.valid_access_free_weak_2
+  Mem.valid_access_free_weak_inv_1
+  Mem.valid_access_free_weak_inv_2
+  Mem.unchanged_on_refl
+: mem.
